theories/proofmode/HNorm.v
@@ -1,0 +1,63 @@
+From CRIS.proofmode Require Import HNormClasses.
+From CRIS.common Require Import Common.
+
+(*** head normalization tactic ***)
+(*
+  itree term        t
+  ktree term        k
+  stuck term        s ::= opaque term
+                        | s >>= k
+                        | ↥ s
+                        | ↧ s
+                        | ░ s
+  head normal term  v ::= Ret x
+                        | Tau t
+                        | vis e k
+                        | assumeK P t
+                        | guaranteeK P t
+                        | unwrapUK x k
+                        | unwrapNK x k
+                        | RealUpdateK pre post k
+                        | SBRed.putSB imports scopes k v cont
+                        | SBRed.getSB imports scopes k cont
+                        | SBRed.callSB imports scopes f a cont
+                        | SBRed.spawnSB imports scopes f a cont
+                        | s
+ *)
+
+(* Opaque ReSum blocks instance resolution occasionally *)
+Typeclasses Transparent ReSum.
+
+(* Keep the wrapper heads distinct from their generic [Vis]/[bind] forms
+   during typeclass search.  In particular, [unwrapUK] and [unwrapNK] stay
+   transparent so their [Some] cases can reduce to [Ret]. *)
+Typeclasses Opaque assumeK guaranteeK RealUpdateK.
+
+Ltac _hnorm_itr :=
+  try (notypeclasses refine (HNormExpand_apply _ _); [tc_solve|]);
+  tryif notypeclasses refine (HNormContext_apply _ _ _); [tc_solve|] then
+    lazymatch goal with
+    | |- HNormContextRes ?K ?b ?b' ?rhs =>
+        econstructor;
+        [ _hnorm_itr
+        | tryif notypeclasses refine (@HNormReduce_apply _ _ K b' _ _ _ _ _); [tc_solve|] then
+            lazymatch goal with
+            | |- HNormReduceRes ?b true ?rhs =>
+                econstructor; simpl; _hnorm_itr
+            | |- HNormReduceRes ?b false ?rhs =>
+                econstructor; reflexivity
+            end
+          else
+            reflexivity
+        ]
+    end
+  else
+    reflexivity.
+
+Ltac hnorm_itr :=
+  etransitivity;
+  [ _hnorm_itr
+  | s;
+    try (notypeclasses refine (HNormFinish_apply _ _); [tc_solve|]);
+    reflexivity
+  ].
